books/arithmetic-4/lib/basic-ops/banner.lisp
@@ -1,0 +1,32 @@
+
+;;;;;;;;;;;;;;;;;;;;;;;;;;;;;;;;;;;;;;;;;;;;;;;;;;;;;;;;;;;;;;;;;
+;;;
+;;; banner.lisp
+;;;
+;;; This file contains a message about how to enable non-linear
+;;; arithmetic.  It is displayed upon including this library.  In
+;;; order to avoid seeing the message twice, be sure that there is no
+;;; compiled file for top.lisp.  The standard "make" procedure ensures
+;;; this through top.acl2.
+;;;
+;;;;;;;;;;;;;;;;;;;;;;;;;;;;;;;;;;;;;;;;;;;;;;;;;;;;;;;;;;;;;;;;;
+
+;;;;;;;;;;;;;;;;;;;;;;;;;;;;;;;;;;;;;;;;;;;;;;;;;;;;;;;;;;;;;;;;;
+
+(in-package "ACL2")
+
+;;;;;;;;;;;;;;;;;;;;;;;;;;;;;;;;;;;;;;;;;;;;;;;;;;;;;;;;;;;;;;;;;
+
+(value-triple
+ (cw "~%To turn on non-linear arithmetic, execute :~|~%~Y02~|~%~
+      or :~|~%~Y12~|~%~
+      See the README for more about non-linear arithmetic and ~
+      general information about using this library.~|~%~%"
+     '(set-default-hints '((nonlinearp-default-hint
+                            stable-under-simplificationp
+			    hist pspv)))
+     '(set-default-hints '((nonlinearp-default-hint++ 
+			   id stable-under-simplificationp
+			   hist nil)))
+     nil)
+ :on-skip-proofs t)
