books/arithmetic-4/lib/basic-ops/dynamic-e-d.lisp
@@ -1,0 +1,94 @@
+
+;;;;;;;;;;;;;;;;;;;;;;;;;;;;;;;;;;;;;;;;;;;;;;;;;;;;;;;;;;;;;;;;;
+;;;
+;;; dynamic-e-d.lisp
+;;;
+;;; This book contains a custom keyword hint which allows enabling and
+;;; disabling of rules in a dynamic environment.  That is, the
+;;; enabling and disabling is done relative to the active theory at
+;;; the goal for which the hint applies, rather than the active theory
+;;; at the time the proof request was submitted.  Thus, one can do,
+;;; for example:
+;;;
+;;; :hints (("Goal"  :dynamic-e/d (((:rewrite foo))()))
+;;;         ("Goal'" :dynamic-e/d (((:rewrite bar))()))
+;;;
+;;; and have both foo and bar enabled at Goal'.  The effects of the
+;;; :dynamic-e/d hints are cumulative.
+;;;
+;;; The argument to :dynamic-e/d should be a pair of lists:
+;;; (<runes to enable> <runes to disable>).  Either list may be empty.
+;;; Otherwise it should be a list of runes.  (The summary of rules
+;;; used at the end of a proof effort is a list of runes.)
+;;;
+;;; Improvements to the error handling, or generalizing the operations
+;;; so that the two lists can look like those for
+;;; :in-theory (e/d <enable list> <disable list>)
+;;; is most welcome.
+;;;
+;;;;;;;;;;;;;;;;;;;;;;;;;;;;;;;;;;;;;;;;;;;;;;;;;;;;;;;;;;;;;;;;;
+
+(in-package "ACL2")
+
+(table acl2-defaults-table :state-ok t)
+
+;;;;;;;;;;;;;;;;;;;;;;;;;;;;;;;;;;;;;;;;;;;;;;;;;;;;;;;;;;;;;;;;;
+
+;;; We grab the theory active at the time the hint is encountered.
+;;; The theory returned is a list of all the enabled runes.
+
+(defun get-current-dynamic-theory (pspv world)
+  (declare (xargs :mode :program))
+  ;; We grab the enabled structure from the pspv, and check for the
+  ;; index-of-last-enabling.  This index is the number of the rune at
+  ;; the time of the last in-theory event, and the enabled structure
+  ;; is current as of this index.  The function enabled-runep
+  ;; considers a rune to be enabled if it is in the enabled structure,
+  ;; or if it's index is greater than the index-of-last-enabling.  See
+  ;; enabled-runep.
+  (let* ((ens (access rewrite-constant
+		      (access prove-spec-var pspv 
+			      :rewrite-constant)
+		      :current-enabled-structure))
+	 (ens-index (access enabled-structure
+			    ens
+			    :index-of-last-enabling)))
+    (if (equal ens-index
+	       (+ -1 (get-next-nume world)))
+	;; Since the index-of-last-enabling is, in fact, that of the
+	;; last rune admited, the ens is up to date.  So we use it to
+	;; get our list of currently active runes.
+	;;
+	;;; In particular, this will be true if there has been an
+	;;; :in-theory hint seen earlier in the proof attempt.
+	(strip-cdrs (cdr (access enabled-structure 
+				 ens
+				 :theory-array)))
+      ;; The ens is not up to date.  We therefore use the theory
+      ;; active at the start of the proof.
+      (current-theory-fn :here world))))
+
+(defun dynamic-e/d (e/d keyword-alist pspv world state)
+  (declare (xargs :mode :program))
+  (let ((enable (car e/d))
+	(disable (cadr e/d)))
+    ;; We should check that the values supplied to enable and disable
+    ;; are lists of runes as expected.
+    (let* ((old-theory (get-current-dynamic-theory pspv world))
+	   ;; should I use set-union-equal?  Append seems sufficient.
+	   (new-theory (set-difference-equal (append enable
+						     old-theory)
+					     disable)))
+      (if (member-equal :in-theory keyword-alist)
+	  ;; Improve the error message, or decide what we should do in
+	  ;; this case.
+	  (er soft 'dynamic-e/d "It is not yet clear to me how dynamic-e/d ~
+                                 should interact with user supplied :in-theory ~
+                                 hints.  We therefore give up.")
+	(let ((new-keyword-alist (splice-keyword-alist :dynamic-e/d
+						       `(:in-theory ',new-theory)
+						       keyword-alist)))
+	  (mv nil new-keyword-alist state))))))
+
+(add-custom-keyword-hint :dynamic-e/d
+			 (dynamic-e/d val keyword-alist pspv world state))
