books/arithmetic-4/lib/floor-mod/floor-mod-helper.lisp
@@ -1,0 +1,164 @@
+;;;;;;;;;;;;;;;;;;;;;;;;;;;;;;;;;;;;;;;;;;;;;;;;;;;;;;;;;;;;;;;;;
+;;;
+;;; floor-mod-helper.lisp
+;;;
+;; This book contains some messy proofs which I want to hide.
+;; There is probably nothing to be gained by looking at it.
+;;;
+;;;;;;;;;;;;;;;;;;;;;;;;;;;;;;;;;;;;;;;;;;;;;;;;;;;;;;;;;;;;;;;;;
+
+;;;;;;;;;;;;;;;;;;;;;;;;;;;;;;;;;;;;;;;;;;;;;;;;;;;;;;;;;;;;;;;;;
+
+(IN-PACKAGE "ACL2")
+
+;;;;;;;;;;;;;;;;;;;;;;;;;;;;;;;;;;;;;;;;;;;;;;;;;;;;;;;;;;;;;;;;;
+
+(table acl2-defaults-table :state-ok t)
+
+(local
+ (include-book "../basic-ops/top"))
+
+(local
+ (include-book "floor-mod-basic"))
+
+(local
+ (include-book "forcing-types"))
+
+(local
+ (SET-DEFAULT-HINTS '((NONLINEARP-DEFAULT-HINT++ ID STABLE-UNDER-SIMPLIFICATIONP
+						 HIST NIL))))
+
+;;;;;;;;;;;;;;;;;;;;;;;;;;;;;;;;;;;;;;;;;;;;;;;;;;;;;;;;;;;;;;;;;
+
+(encapsulate
+ ()
+
+ (local
+  (defthm floor-sum-cases-helper-a
+    (implies (and (rationalp (/ x z))
+		  (rationalp (/ y z)))
+	     (<= (floor (+ x y) z)
+		 (cond ((not (acl2-numberp z))
+			0)
+		       ((equal z 0)
+			0)
+		       ((< 0 z)
+			(if (< (+ (mod x z) (mod y z)) z)
+			    (+ (floor x z) (floor y z))
+			  (+ 1 (floor x z) (floor y z))))
+		       (t
+			(if (< z (+ (mod x z) (mod y z)))
+			    (+ (floor x z) (floor y z))
+			  (+ 1 (floor x z) (floor y z)))))))
+    :hints (("Goal" :in-theory (enable mod)))))
+
+ (local
+  (defthm floor-sum-cases-helper-b
+    (implies (and (rationalp (/ x z))
+		  (rationalp (/ y z)))
+	     (<= (cond ((not (acl2-numberp z))
+			0)
+		       ((equal z 0)
+			0)
+		       ((< 0 z)
+			(if (< (+ (mod x z) (mod y z)) z)
+			    (+ (floor x z) (floor y z))
+			  (+ 1 (floor x z) (floor y z))))
+		       (t
+			(if (< z (+ (mod x z) (mod y z)))
+			    (+ (floor x z) (floor y z))
+			  (+ 1 (floor x z) (floor y z)))))
+		 (floor (+ x y) z)))
+    :hints (("Goal" :in-theory (enable mod)))))
+
+ (local
+  (in-theory (disable floor-sum-cases-helper-a
+		      floor-sum-cases-helper-b)))
+
+ (defthm |(floor (+ x y) z)|
+   (implies (and (rationalp (/ x z))
+		 (rationalp (/ y z)))
+	    (equal (floor (+ x y) z)
+		   (cond ((not (acl2-numberp z))
+			  0)
+			 ((equal z 0)
+			  0)
+			 ((< 0 z)
+			  (if (< (+ (mod x z) (mod y z)) z)
+			      (+ (floor x z) (floor y z))
+			    (+ 1 (floor x z) (floor y z))))
+			 (t
+			  (if (< z (+ (mod x z) (mod y z)))
+			      (+ (floor x z) (floor y z))
+			    (+ 1 (floor x z) (floor y z)))))))
+   :hints (("Goal" :use ((:instance floor-sum-cases-helper-a)
+			 (:instance floor-sum-cases-helper-b)))))
+
+ )
+
+(defthm |(mod (+ x y) z)|
+  (implies (and (rationalp (/ x z))
+                (rationalp (/ y z)))
+           (equal (mod (+ x y) z)
+		  (if (<= 0 z)
+		      (if (< (+ (mod x z) (mod y z)) z)
+			  (+ (mod x z) (mod y z))
+			(+ (mod x z) (mod y z) (- z)))
+		    (if (< z (+ (mod x z) (mod y z)))
+			(+ (mod x z) (mod y z))
+		      (+ (mod x z) (mod y z) (- z))))))
+  :hints (("Goal" :in-theory (enable mod))))
+
+
+
+
+
+
+
+
+(encapsulate
+ ()
+
+ (local
+  (defthm crock-xxx33-helper
+    (implies (and (acl2-numberp md0)
+		  (acl2-numberp j)
+		  (acl2-numberp z)
+		  (not (equal z 0))
+		  (equal 0 (+ md0 (* j z))))
+	     (equal (* md0 (/ z)) (- j)))
+    :rule-classes nil))
+
+ (local
+  (defthm crock-xxx33a
+    (implies (and (acl2-numberp md0)
+		  (integerp j)
+		  (acl2-numberp z)
+		  (not (equal z 0))
+		  (equal 0 (+ md0 (* j z))))
+	     (integerp (* md0 (/ z))))
+    :hints (("Goal" :use crock-xxx33-helper))))
+ 
+ (defthm rewrite-floor-mod
+   (implies (and ;(acl2-numberp x)
+		 ;(acl2-numberp y)
+		 (rationalp (/ x y))
+		 (rationalp (/ x z))
+		 (rationalp (/ (mod x y) z))
+		 (equal i (/ y z))
+		 (integerp i))
+	    (equal (floor (mod x y) z)
+		   (- (floor x z) (* i (floor x y))))))
+
+ (defthm rewrite-mod-mod
+   (implies (and (acl2-numberp z)
+		 (rationalp (/ x y))
+		 (rationalp (/ x z))
+		 (not (equal z 0))
+		 (equal i (/ y z))
+		 (integerp i))
+	    (equal (mod (mod x y) z)
+		   (mod x z)))
+   :hints (("Subgoal 1" :in-theory (enable mod)))
+   :otf-flg t)
+ )
