books/arithmetic-4/lib/floor-mod/more-floor-mod.lisp
@@ -1,0 +1,410 @@
+;;;;;;;;;;;;;;;;;;;;;;;;;;;;;;;;;;;;;;;;;;;;;;;;;;;;;;;;;;;;;;;;;
+;;;
+;;; more-floor-mod.lisp
+;;;
+;;; Here are some more theorems about floor and mod.
+;;;
+;;;;;;;;;;;;;;;;;;;;;;;;;;;;;;;;;;;;;;;;;;;;;;;;;;;;;;;;;;;;;;;;;
+
+(in-package "ACL2")
+
+;;;;;;;;;;;;;;;;;;;;;;;;;;;;;;;;;;;;;;;;;;;;;;;;;;;;;;;;;;;;;;;;;
+
+(include-book "../basic-ops/top")
+
+(include-book "floor-mod")
+
+(include-book "floor-mod-basic")
+
+;;; We want these to be the first rules seen:
+
+(include-book "if-normalization")
+
+(include-book "forcing-types")
+
+(SET-DEFAULT-HINTS
+     '((NONLINEARP-DEFAULT-HINT++ ID STABLE-UNDER-SIMPLIFICATIONP
+                                  HIST NIL)))
+
+;;;;;;;;;;;;;;;;;;;;;;;;;;;;;;;;;;;;;;;;;;;;;;;;;;;;;;;;;;;;;;;;;
+
+(local
+ (defthm extra-intp-thm-1
+   (IMPLIES (AND (INTEGERP (* (/ I) (/ J) X))
+              (RATIONALP X)
+              (INTEGERP I)
+              (INTEGERP J)
+              (NOT (EQUAL J 0)))
+         (INTEGERP (* (/ I) X)))
+   :hints (("Goal" :use (:instance
+			 (:theorem
+			  (implies (and (integerp x)
+					(integerp y))
+				   (integerp (* x y))))
+			 (x (* (/ I) (/ J) X))
+			 (y j))))))
+
+(local
+ (defthm extra-intp-thm-3
+   (IMPLIES (AND (INTEGERP (* (/ I) (/ J) X))
+		 (RATIONALP X)
+		 (INTEGERP I)
+		 (INTEGERP J))
+	    (INTEGERP (* (/ J) (FLOOR X I))))
+   :hints (("Goal" :cases ((equal j 0))))))
+
+(defthm foo   ;;; OK
+  (implies (and (integerp x)
+                ;(<= 0 x)
+                (rationalp r)
+                (<= 0 r)
+                (< r 1)
+                (integerp i)
+                (< 0 i)
+		)
+           (equal (floor (+ x r) i)
+                  (floor x i))))
+
+;;; Move with floor-floor-integer?
+
+(defthm mod-x-i*j   ;;; OK
+    (implies
+     (and (> i 0)
+	  (> j 0)
+	  (force (integerp i))
+	  (force (integerp j))
+	  (force (real/rationalp x)))
+     (equal (mod x (* i j))
+	    (+ (mod x i) (* i (mod (floor x i) j))))))
+
+;;; Beter version:
+
+(local
+ (defthm this-is-odd
+  (IMPLIES (AND (INTEGERP I)
+		(INTEGERP J)
+		(RATIONALP X)
+		(< J 0)
+		(NOT (INTEGERP (* (/ I) (/ J) X)))
+		(INTEGERP (* (/ J) (FLOOR X I))))
+	   (EQUAL (MOD X (* I J))
+		  (+ (* i j) (mod x i))))))
+
+;;; Is this a good rule?
+;;; It breaks the proof of mod-prod.
+
+(defthmd mod-x-i*j-x-2 ;;; OK
+  (implies (and (force (integerp i))
+		(force (integerp j))
+		(force (real/rationalp x)))
+   (equal (mod x (* i j))
+	  (cond ((and (< j 0)
+		      (not (integerp (* (/ i) (/ j) x)))
+		      (integerp (* (/ j) (floor x i))))
+		 (+ (* i j) (mod x i)))
+		(t
+		 (+ (mod x i) (* i (mod (floor x i) j)))))))
+  :hints (("Subgoal 3" :use (:instance this-is-odd))
+	  ("Subgoal 2" :cases ((equal j 0))))
+  :otf-flg t)
+
+;;; Subsumed by the above?
+
+(defthm mod-x+i*k-i*j
+  (implies
+   (and (force (real/rationalp x))
+	(force (integerp i))
+	(force (integerp j))
+	(force (integerp k))
+	(< 0 i)
+	(< 0 j)
+	(<= 0 x)
+	(< x i))
+  (equal (mod (+ x (* i k)) (* i j))
+	 (+ x (* i (mod k j))))))
+
+;;; Subsumed by floor-floor-integer?
+
+(defthm floor-x+i*k-i*j
+  (implies
+   (and (force (real/rationalp x))
+	(force (integerp i))
+	(force (integerp j))
+	(force (integerp k))
+	(< 0 i)
+	(< 0 j)
+	(<= 0 x)
+	(< x i))
+   (equal (floor (+ x (* i k)) (* i j))
+	  (floor k j))))
+
+(defthm floor-equal-i-over-j-rewrite   ;;; OK
+  (implies (and (case-split (not (equal j 0)))
+                (case-split (rationalp i))
+                (case-split (rationalp j))
+                )
+           (equal (equal (* j (floor i j)) i)
+                  (integerp (* i (/ j))))))
+
+(defthm mod-plus-mod-2   ;;; OK
+  (implies (and (integerp a)
+                (integerp b)
+		(integerp n))
+           (iff (= (mod (+ a b) n) (mod a n))
+                (= (mod b n) 0)))
+  :rule-classes ())
+
+(defthmd mod-mult-n   ;;; OK
+  (equal (mod (* a n) n)
+         (* n (mod a 1))))
+
+
+
+(defthm mod-theorem-one-a   ;;; OK
+  (implies (and (rationalp a)
+		(integerp b)
+		(rationalp n)
+		(not (equal n 0)))
+	   (equal (mod (* (mod a n) b) n)
+		  (mod (* a b) n))))
+
+(defthm mod-theorem-one-b   ;;; OK
+  (implies (and (rationalp a)
+		(integerp b)
+		(rationalp n)
+		(not (equal n 0)))
+	   (equal (mod (* b (mod a n)) n)
+		  (mod (* a b) n))))
+
+(encapsulate ()
+
+ (local
+  (defun ind-fn (i)
+    (if (zp i)
+	t
+      (ind-fn (+ -1 i)))))
+
+ ;; Robert Krug writes:  This hint took some knowledge about the
+ ;; library, but it is described in the README.  If you can suggest a
+ ;; way to make this more easily accessable, I would be interested in
+ ;; hearing it.
+
+ (local
+  (scatter-exponents))
+
+ ;; Robert Krug writes:  I believe I could prove this or an
+ ;; equivalent one using instances of mod-theorem-one-a or
+ ;; mod-theorem-one-b, but this is what I tried first.
+
+ ;; RBK: Fix this proof.  72 generalizations and 96 destructor
+ ;; eliminations!
+
+ (local
+  (defthm mod-theorem-two-helper-helper
+    (IMPLIES (AND (NOT (ZP I))
+		  (EQUAL (MOD (EXPT A I) N)
+			 (MOD (EXPT (MOD A N) I) N))
+		  (INTEGERP A)
+		  (integerp b)
+		  (INTEGERP N)
+		  (NOT (EQUAL N 0)))
+	     (EQUAL (MOD (* b (EXPT (MOD A N) I)) N)
+		    (MOD (* b (EXPT A I)) N)))
+    :hints (("Goal" :induct (ind-fn b)))))
+
+ ;; Robert Krug writes:  This helper, and ones like it, irritate me.
+ ;; ACL2 failed to prove theorem two, with the subgoal:
+
+ ;; (IMPLIES (AND (NOT (ZP I))
+ ;;               (EQUAL (MOD (EXPT A (+ -1 I)) N)
+ ;;                      (MOD (EXPT (MOD A N) (+ -1 I)) N))
+ ;;               (INTEGERP A)
+ ;;               (INTEGERP N)
+ ;;               (NOT (EQUAL N 0)))
+ ;;          (EQUAL (MOD (EXPT (MOD A N) I) N)
+ ;;                 (MOD (EXPT A I) N)))
+
+ ;; but (EXPT A (+ -1 I)) expand to (* (/ A) (EXPT A I)) and
+ ;; thus introduces division which is always harder to reason
+ ;; about than multiplication.  It would be nice if ACL2 could
+ ;; induct with a base case of I and an inductive case of (+ 1 I),
+ ;; rather than using a base case of (+ -1 I) and an indictive
+ ;; case of I.  But this is not going to happen.
+
+ (local
+  (defthm mod-theorem-two-helper
+    (IMPLIES (AND (NOT (ZP I))
+		  (EQUAL (MOD (EXPT A I) N)
+			 (MOD (EXPT (MOD A N) I) N))
+		  (INTEGERP A)
+		  (INTEGERP N)
+		  (NOT (EQUAL N 0)))
+	     (EQUAL (MOD (EXPT (MOD A N) (+ 1 I)) N)
+		    (MOD (EXPT A (+ 1 I)) N)))))
+
+ (local
+  (gather-exponents))
+
+ (defthm mod-theorem-two
+   (implies (and (integerp a)
+		 (integerp i)
+		 (<= 0 i)
+		 (integerp n)
+		 (not (equal n 0)))
+	    (equal (mod (expt (mod a n) i) n)
+		   (mod (expt a i) n)))
+   :hints (("Goal" :induct (ind-fn i)
+	    :do-not '(generalize))
+	   ("Subgoal *1/2''" :cases ((equal i 1)))
+	   ("Subgoal *1/2.2" :use (:instance mod-theorem-two-helper
+					     (i (+ -1 i)))
+	    :in-theory (disable mod-theorem-two-helper))))
+
+ )
+
+(defthm two-xxx   ;;; OK
+  (IMPLIES (AND (integerp x)
+		(< 0 x)
+		(INTEGERP N)
+		(<= 0 N)
+		(NOT (INTEGERP (* 1/2 X))))
+	   (EQUAL (+ 1
+		     (* 2 (MOD (FLOOR X 2) (EXPT 2 n))))
+		  (MOD X (EXPT 2 (+ 1 N)))))
+  :hints (("Goal" :do-not '(generalize)
+	   :do-not-induct t))
+  :otf-flg t)
+
+
+
+(defthm mod-theorem-three
+  (implies (and (integerp a)
+		(integerp i)
+		(<= 0 i)
+		(integerp n)
+		(not (equal n 0))
+		(integerp x))
+	   (equal (mod (* x (expt (mod a n) i)) n)
+		  (mod (* x (expt a i)) n)))
+  :hints (("Goal" :use ((:instance mod-theorem-one-a
+				  (a (expt (mod a n) i))
+				  (b x))
+			(:instance mod-theorem-one-a
+				  (a (expt a i))
+				  (b x)))
+	          :in-theory (disable mod-theorem-one-a
+                                      mod-theorem-one-b))))
+
+
+
+(defthm mod-mult-2
+  (implies (integerp a)
+           (equal (mod (* a n) n)
+                  0))
+  :hints (("Goal" :cases ((equal n 0)))))
+
+(defthm mod-prod
+  (implies (and (rationalp m)
+                (rationalp n)
+                (rationalp k)
+                )
+           (equal (mod (* k m) (* k n))
+                  (* k (mod m n))))
+  :otf-flg t)
+
+(defthm mod-mult
+    (implies (and (integerp a)
+                  (rationalp m)
+		  (rationalp n))
+	     (equal (mod (+ m (* a n)) n)
+		    (mod m n))))
+
+
+;;; floor rule like below also?
+
+(defthm mod-sums-cancel-1
+  (implies (and (case-split (<= 0 y))
+                (case-split (rationalp k))
+                (case-split (rationalp y))
+                (case-split (rationalp x1))
+                (case-split (rationalp x2))
+                )
+           (equal (equal (mod (+ k x1) y) (mod (+ k x2) y))
+                  (equal (mod x1 y) (mod x2 y)))))
+
+(defthm  |(equal (mod a n) (mod b n))|
+  (implies (and (integerp (+ (* a (/ n)) (- (* b (/ n)))))
+		(rationalp a)
+		(rationalp b)
+		(rationalp n)
+		(not (equal n 0)))
+	   (equal (equal (mod a n) (mod b n))
+		  t))
+  :hints (("Goal" :use (:instance mod-zero
+				  (x (+ a (- b)))
+				  (y n))
+	          :in-theory (e/d ()
+				  (mod-zero)))))
+
+;;; Will this base case for the above be caught, or should we have a
+;;; second rule?
+
+;;; Add default-xxx rules 
+;;; add if normalization rules
+
+;; RBK:!!! Separate rules into units --- i.e. no multiple corr.s
+
+;; (equal (equal (floor a (expt 2 i)) (floor b (expt 2 j))
+;;        (equal (floor a (expt (...)) b)))
+
+#|
+(defthm thm-1
+    (implies (and (integerp a)
+                  (integerp b)
+                  (integerp n))
+             (equal (MOD (+ (* B (FIBONACCI (+ -2 N)))
+                            (* (FIBONACCI (+ -2 N))
+                               (MOD (+ A B) 4294967296))
+                            (* (FIBONACCI (+ -3 N))
+                               (MOD (+ A B) 4294967296)))
+                         4294967296)
+                    (MOD (+ (* A (FIBONACCI (+ -2 N)))
+                            (* A (FIBONACCI (+ -3 N)))
+                            (* B (FIBONACCI (+ -3 N)))
+                            (* 2 B (FIBONACCI (+ -2 N))))
+                         4294967296)))
+  :hints (("Goal" :in-theory (enable mod))))
+|#
+
+
+#|
+; Something like the following rules are missing from my library.
+; The versions below do not seem particularly good, but I have
+; not given it much thought yet.
+
+;;; Make a mod-floor rule like floor-mod
+
+;Basic idea: mod chops off some high bits from x and fl chops off some
+;low bits.  We can do the chops in either order.
+
+
+(defthm crock-628
+  (equal (floor 0 x)
+	 0))
+
+
+(defthm mod-pull-inside-fl-shift
+   (implies (and ;no hyp about x
+	     (rationalp x)
+             (integerp i)
+             (integerp j)
+             )
+            (equal (mod (floor x (expt 2 j))
+                        (expt 2 i))
+                   (floor (mod x (expt 2 (+ i j)))
+                          (expt 2 j))))
+   :hints (("Goal" :cases ((<= 0 i))))
+   :otf-flg t)
+
+
+|#
