books/make-event/macros-skip-proofs-include.lisp
@@ -16,8 +16,6 @@
      ((LOCAL-FN (X) T))
      (LOCAL (DEFUN LOCAL-FN (X) X))
      (RECORD-EXPANSION (LOCAL (MAKE-EVENT '(DEFUN FOO1 (X) X)))
-; Change for v3-4:
-;                      (LOCAL (DEFUN FOO1 (X) X)))
                        (LOCAL (value-triple :elided)))
      (RECORD-EXPANSION
       (MY-MAC (SKIP-PROOFS (MAKE-EVENT '(DEFUN FOO2 (X) X)
@@ -42,12 +40,8 @@
 
 (include-book "misc/file-io" :dir :system)
 
-; Uncomment the following when updating to v3-4, and also perhaps remove
-; comment above v3-4 above.
-#||
 (must-succeed
  (er-let* ((forms (read-list "macros-skip-proofs.cert" 'top state)))
           (let ((erp (not (equal (cadr (member-eq :expansion-alist forms))
                                  *macros-expansion-alist*))))
             (mv erp nil state))))
-||#
